<?xml version="1.0"?>


<!DOCTYPE rdf:RDF [
    <!ENTITY owl "http://www.w3.org/2002/07/owl#" >
    <!ENTITY fivestars "http://purl.org/spar/fivestars/" >
    <!ENTITY dc "http://purl.org/dc/elements/1.1/" >
    <!ENTITY xsd "http://www.w3.org/2001/XMLSchema#" >
    <!ENTITY rdfs "http://www.w3.org/2000/01/rdf-schema#" >
    <!ENTITY rdf "http://www.w3.org/1999/02/22-rdf-syntax-ns#" >
]>


<rdf:RDF xmlns="http://purl.org/spar/fivestars/"
     xml:base="http://purl.org/spar/fivestars/"
     xmlns:dc="http://purl.org/dc/elements/1.1/"
     xmlns:rdfs="http://www.w3.org/2000/01/rdf-schema#"
     xmlns:owl="http://www.w3.org/2002/07/owl#"
     xmlns:xsd="http://www.w3.org/2001/XMLSchema#"
     xmlns:rdf="http://www.w3.org/1999/02/22-rdf-syntax-ns#"
     xmlns:fivestars="http://purl.org/spar/fivestars/">
    <owl:Ontology rdf:about="http://purl.org/spar/fivestars">
        <owl:versionInfo rdf:datatype="&xsd;string">1.0</owl:versionInfo>
        <owl:versionIRI rdf:resource="http://purl.org/spar/fivestars/2012-01-16"/>
        <dc:creator rdf:datatype="&xsd;string">David Shotton</dc:creator>
        <dc:date>2012-01-16</dc:date>
        <dc:title xml:lang="en">The Five Stars of Online Research Articles Ontology (FiveStars)</dc:title>
        <rdfs:comment xml:lang="en">The Five Stars of Online Research Articles Ontology (FiveStars) is an ontology written in OWL 2 DL to enable characterization of the five attributes of an online journal article - peer review, open access, enriched content, available datasets and machine-readable metadata.

**URL:** http://purl.org/spar/fivestars

**Creators**: [David Shotton](http://orcid.org/0000-0001-5506-523X)

**License:** [Creative Commons Attribution 4.0 International](https://creativecommons.org/licenses/by/4.0/legalcode)

**Website:** http://www.sparontologies.net/ontologies/fivestars

**Cite as:** Shotton, D. (2012). The Five Stars of Online Journal Articles - a Framework for Article Evaluation. In D-Lib Magazine, 18 (1/2). DOI: https://doi.org/10.1045/january2012-shotton  </rdfs:comment>
        <dc:description xml:lang="en">The Five Stars of Online Research Articles Ontology, is an ontology written in OWL 2 DL to enable characterization of the five attributes of an online journal article - peer review, open access, enriched content, available datasets and machine-readable metadata - using the criteria discussed in the paper by David Shotton entitled The Five Stars of Online Journal Articles â€” a Framework for Article Evaluation, published in D-Lib Magazine 18 (1/2) (January/February 2012 issue).  doi: https://doi.org/10.1045/january2012-shotton.

The ontology is simple, consisting only of those data properties required to permit a rating for each of the five stars, and for the paper as a whole, to be recorded as an integer, together with an associated comment.  It is intended for use by publishers and others wishing to encode Five Stars ratings for individual papers in machine-readable form.

Other ontologies, for example DCMI Metadata Terms (http://dublincore.org/documents/dcmi-terms/) and FaBiO, the FRBR-aligned Bibliographic Ontology (http://purl.org/spar/fabio), may be used to describe other aspects of a journal article, e.g. authors, journal name, and publication year.
</dc:description>
        <dc:rights xml:lang="en">This work is distributed under a Creative Commons Attribution License (http://creativecommons.org/licenses/by/4.0/).</dc:rights>
    </owl:Ontology>
    


    <!-- 
    ///////////////////////////////////////////////////////////////////////////////////////
    //
    // Annotation properties
    //
    ///////////////////////////////////////////////////////////////////////////////////////
     -->

    <owl:AnnotationProperty rdf:about="&owl;versionInfo"/>
    <owl:AnnotationProperty rdf:about="&dc;creator"/>
    <owl:AnnotationProperty rdf:about="&dc;contributor"/>
    <owl:AnnotationProperty rdf:about="&owl;priorVersion"/>
    <owl:AnnotationProperty rdf:about="&dc;date"/>
    <owl:AnnotationProperty rdf:about="&rdfs;label"/>
    <owl:AnnotationProperty rdf:about="&dc;description"/>
    <owl:AnnotationProperty rdf:about="&rdfs;comment"/>
    <owl:AnnotationProperty rdf:about="&dc;title"/>
    <owl:AnnotationProperty rdf:about="&dc;rights"/>
    


    <!-- 
    ///////////////////////////////////////////////////////////////////////////////////////
    //
    // Datatypes
    //
    ///////////////////////////////////////////////////////////////////////////////////////
     -->

    


    <!-- 
    ///////////////////////////////////////////////////////////////////////////////////////
    //
    // Object Properties
    //
    ///////////////////////////////////////////////////////////////////////////////////////
     -->

    


    <!-- http://www.w3.org/2002/07/owl#topObjectProperty -->

    <owl:ObjectProperty rdf:about="&owl;topObjectProperty"/>
    


    <!-- 
    ///////////////////////////////////////////////////////////////////////////////////////
    //
    // Data properties
    //
    ///////////////////////////////////////////////////////////////////////////////////////
     -->

    


    <!-- http://purl.org/spar/fivestars/availableDatasetsRatingComment -->

    <owl:DatatypeProperty rdf:about="&fivestars;availableDatasetsRatingComment">
        <rdfs:comment xml:lang="en">Comment explaining Five Stars ratings given to journal artice relating to available datasets.</rdfs:comment>
    </owl:DatatypeProperty>
    


    <!-- http://purl.org/spar/fivestars/enhancedContentRatingComment -->

    <owl:DatatypeProperty rdf:about="&fivestars;enhancedContentRatingComment">
        <rdfs:comment xml:lang="en">Comment explaining Five Stars ratings given to journal artice relating to enhanced content.</rdfs:comment>
    </owl:DatatypeProperty>
    


    <!-- http://purl.org/spar/fivestars/hasAvailableDatasetsRating -->

    <owl:DatatypeProperty rdf:about="&fivestars;hasAvailableDatasetsRating">
        <rdfs:comment xml:lang="en">Integer rating (from 0 to 4) given to journal artice for available datasets.</rdfs:comment>
        <rdfs:range rdf:resource="&xsd;nonNegativeInteger"/>
    </owl:DatatypeProperty>
    


    <!-- http://purl.org/spar/fivestars/hasEnhancedContentRating -->

    <owl:DatatypeProperty rdf:about="&fivestars;hasEnhancedContentRating">
        <rdfs:comment xml:lang="en">Integer rating (from 0 to 4) given to journal artice for enhanced content.</rdfs:comment>
        <rdfs:range rdf:resource="&xsd;nonNegativeInteger"/>
    </owl:DatatypeProperty>
    


    <!-- http://purl.org/spar/fivestars/hasMachine-readableMetadataRating -->

    <owl:DatatypeProperty rdf:about="&fivestars;hasMachine-readableMetadataRating">
        <rdfs:comment xml:lang="en">Integer rating (from 0 to 4) given to journal artice for machine-readable metadata.</rdfs:comment>
        <rdfs:range rdf:resource="&xsd;nonNegativeInteger"/>
    </owl:DatatypeProperty>
    


    <!-- http://purl.org/spar/fivestars/hasOpenAccessRating -->

    <owl:DatatypeProperty rdf:about="&fivestars;hasOpenAccessRating">
        <rdfs:comment xml:lang="en">Integer rating (from 0 to 4) given to journal artice for open access.</rdfs:comment>
        <rdfs:range rdf:resource="&xsd;nonNegativeInteger"/>
    </owl:DatatypeProperty>
    


    <!-- http://purl.org/spar/fivestars/hasOverallFiveStarsRating -->

    <owl:DatatypeProperty rdf:about="&fivestars;hasOverallFiveStarsRating">
        <rdfs:comment xml:lang="en">Overall Five stars rating (on integer scale from from 0 to 20) given to journal artice, obtained by summing the individual ratings given for each of the Five Stars of Online Journal Articles.</rdfs:comment>
        <rdfs:range rdf:resource="&xsd;nonNegativeInteger"/>
    </owl:DatatypeProperty>
    


    <!-- http://purl.org/spar/fivestars/hasPeerReviewRating -->

    <owl:DatatypeProperty rdf:about="&fivestars;hasPeerReviewRating">
        <rdfs:comment xml:lang="en">Integer rating (from 0 to 4) given to journal artice for peer review.</rdfs:comment>
        <rdfs:range rdf:resource="&xsd;nonNegativeInteger"/>
    </owl:DatatypeProperty>
    


    <!-- http://purl.org/spar/fivestars/machine-readableMetadataRatingComment -->

    <owl:DatatypeProperty rdf:about="&fivestars;machine-readableMetadataRatingComment">
        <rdfs:comment xml:lang="en">Comment explaining Five Stars ratings given to journal artice relating to machine-readable metadata.</rdfs:comment>
    </owl:DatatypeProperty>
    


    <!-- http://purl.org/spar/fivestars/openAccessRatingComment -->

    <owl:DatatypeProperty rdf:about="&fivestars;openAccessRatingComment">
        <rdfs:comment xml:lang="en">Comment explaining Five Stars ratings given to journal artice relating to open access.</rdfs:comment>
    </owl:DatatypeProperty>
    


    <!-- http://purl.org/spar/fivestars/overallFiveStarsRatingComment -->

    <owl:DatatypeProperty rdf:about="&fivestars;overallFiveStarsRatingComment">
        <rdfs:comment xml:lang="en">Comment on overall Five Stars rating given to journal artice.</rdfs:comment>
    </owl:DatatypeProperty>
    


    <!-- http://purl.org/spar/fivestars/peerReviewRatingComment -->

    <owl:DatatypeProperty rdf:about="&fivestars;peerReviewRatingComment">
        <rdfs:comment xml:lang="en">Comment explaining Five Stars ratings given to journal artice relating to peer review.</rdfs:comment>
    </owl:DatatypeProperty>
</rdf:RDF>



<!-- Generated by the OWL API (version 3.2.3.1824) http://owlapi.sourceforge.net -->

